[CBPV] cleanup

CBPV/CK.lean
@@ -2,6 +2,8 @@ import CBPV.RTC
 import CBPV.Syntax
 import CBPV.Evaluation
 
+open Val Com
+
 namespace CK
 
 inductive F : Type where
@@ -17,34 +19,34 @@ def CK := Com × K
 @[simp]
 def renameK (ξ : Nat → Nat) : K → K
   | [] => []
-  | app v :: k => .app (renameVal ξ v) :: renameK ξ k
-  | letin m :: k => .letin (renameCom (lift ξ) m) :: renameK ξ k
-  | fst :: k => fst :: renameK ξ k
-  | snd :: k => snd :: renameK ξ k
+  | .app v :: k => app (renameVal ξ v) :: renameK ξ k
+  | .letin m :: k => letin (renameCom (lift ξ) m) :: renameK ξ k
+  | .fst :: k => fst :: renameK ξ k
+  | .snd :: k => snd :: renameK ξ k
 
 @[simp]
 def dismantle (n : Com) : K → Com
   | [] => n
-  | app v :: k => dismantle (.app n v) k
-  | letin m :: k => dismantle (.letin n m) k
-  | fst :: k => dismantle (.fst n) k
-  | snd :: k => dismantle (.snd n) k
+  | .app v :: k => dismantle (app n v) k
+  | .letin m :: k => dismantle (letin n m) k
+  | .fst :: k => dismantle (fst n) k
+  | .snd :: k => dismantle (snd n) k
 
 section
 set_option hygiene false
 local infix:40 "⤳" => Step
 inductive Step : CK → CK → Prop where
-  | β {m v k} :     ⟨.lam m, .app v :: k⟩   ⤳ ⟨substCom (v +: .var) m, k⟩
-  | ζ {v m k} :     ⟨.ret v, .letin m :: k⟩ ⤳ ⟨substCom (v +: .var) m, k⟩
-  | ιl {v m n k} :  ⟨.case (.inl v) m n, k⟩ ⤳ ⟨substCom (v +: .var) m, k⟩
-  | ιr {v m n k} :  ⟨.case (.inr v) m n, k⟩ ⤳ ⟨substCom (v +: .var) n, k⟩
-  | π {m k} :       ⟨.force (.thunk m), k⟩  ⤳ ⟨m, k⟩
-  | π1 {m n k} :    ⟨.prod m n, .fst :: k⟩  ⤳ ⟨m, k⟩
-  | π2 {m n k} :    ⟨.prod m n, .snd :: k⟩  ⤳ ⟨n, k⟩
-  | app {m v k} :   ⟨.app m v, k⟩           ⤳ ⟨m, .app v :: k⟩
-  | letin {m n k} : ⟨.letin m n, k⟩         ⤳ ⟨m, .letin n :: k⟩
-  | fst {m k} :     ⟨.fst m, k⟩             ⤳ ⟨m, .fst :: k⟩
-  | snd {m k} :     ⟨.snd m, k⟩             ⤳ ⟨m, .snd :: k⟩
+  | β {m v k} :     ⟨lam m, app v :: k⟩   ⤳ ⟨substCom (v +: var) m, k⟩
+  | ζ {v m k} :     ⟨ret v, letin m :: k⟩ ⤳ ⟨substCom (v +: var) m, k⟩
+  | ιl {v m n k} :  ⟨case (inl v) m n, k⟩ ⤳ ⟨substCom (v +: var) m, k⟩
+  | ιr {v m n k} :  ⟨case (inr v) m n, k⟩ ⤳ ⟨substCom (v +: var) n, k⟩
+  | π {m k} :       ⟨force (thunk m), k⟩  ⤳ ⟨m, k⟩
+  | π1 {m n k} :    ⟨prod m n, fst :: k⟩  ⤳ ⟨m, k⟩
+  | π2 {m n k} :    ⟨prod m n, snd :: k⟩  ⤳ ⟨n, k⟩
+  | app {m v k} :   ⟨app m v, k⟩          ⤳ ⟨m, app v :: k⟩
+  | letin {m n k} : ⟨letin m n, k⟩        ⤳ ⟨m, letin n :: k⟩
+  | fst {m k} :     ⟨fst m, k⟩            ⤳ ⟨m, fst :: k⟩
+  | snd {m k} :     ⟨snd m, k⟩            ⤳ ⟨m, snd :: k⟩
 end
 infix:40 "⤳" => Step
 
@@ -59,56 +61,111 @@ section
 set_option hygiene false
 local infix:40 "⇓" => BStep
 inductive BStep : Com → Com → Prop where
-  | lam {m} : .lam m ⇓ .lam m
-  | ret {v} : .ret v ⇓ .ret v
-  | prod {m₁ m₂} : .prod m₁ m₂ ⇓ .prod m₁ m₂
+  | lam {m} : lam m ⇓ lam m
+  | ret {v} : ret v ⇓ ret v
+  | prod {m₁ m₂} : prod m₁ m₂ ⇓ prod m₁ m₂
   | π {m t} :
     m ⇓ t →
-    ---------------------
-    .force (.thunk m) ⇓ t
+    -------------------
+    force (thunk m) ⇓ t
   | β {n t m v} :
-    n ⇓ .lam m →
-    substCom (v +: .var) m ⇓ t →
-    -----------------------------
-    .app n v ⇓ t
+    n ⇓ lam m →
+    substCom (v +: var) m ⇓ t →
+    ---------------------------
+    app n v ⇓ t
   | ζ {n t v m} :
-    n ⇓ .ret v →
-    substCom (v +: .var) m ⇓ t →
-    -----------------------------
-    .letin n m ⇓ t
+    n ⇓ ret v →
+    substCom (v +: var) m ⇓ t →
+    ---------------------------
+    letin n m ⇓ t
   | ιl {v m₁ m₂ t}:
-    substCom (v +: .var) m₁ ⇓ t →
-    -----------------------------
-    .case (.inl v) m₁ m₂ ⇓ t
+    substCom (v +: var) m₁ ⇓ t →
+    ----------------------------
+    case (inl v) m₁ m₂ ⇓ t
   | ιr {v m₁ m₂ t}:
-    substCom (v +: .var) m₂ ⇓ t →
-    -----------------------------
-    .case (.inr v) m₁ m₂ ⇓ t
+    substCom (v +: var) m₂ ⇓ t →
+    ----------------------------
+    case (inr v) m₁ m₂ ⇓ t
   | π1 {n t m₁ m₂} :
-    n ⇓ .prod m₁ m₂ →
+    n ⇓ prod m₁ m₂ →
     m₁ ⇓ t →
-    -----------
-    .fst n ⇓ t
+    ----------------
+    fst n ⇓ t
   | π2 {n t m₁ m₂} :
-    n ⇓ .prod m₁ m₂ →
+    n ⇓ prod m₁ m₂ →
     m₂ ⇓ t →
-    -----------
-    .snd n ⇓ t
+    ----------------
+    snd n ⇓ t
 end
 infix:40 "⇓" => BStep
 
 @[simp]
 def isTerminal : Com → Prop
-  | .lam _ | .ret _ | .prod _ _ => True
+  | lam _ | ret _ | prod _ _ => True
   | _ => False
 
 end Big
+
+namespace Eq
+
+section
+set_option hygiene false
+local infix:40 "≡" => EqVal
+local infix:40 "≡" => EqCom
+mutual
+inductive EqVal : Val → Val → Prop
+  | var {x} : var x ≡ var x
+  | unit : unit ≡ unit
+  | inl {v w : Val} : v ≡ w → inl v ≡ inl w
+  | inr {v w : Val} : v ≡ w → inr v ≡ inr w
+  | thunk {m n : Com} : m ≡ n → thunk m ≡ thunk n
+  | sym {v w : Val} : w ≡ v → v ≡ w
+  | trans {u v w : Val} : u ≡ v → v ≡ w → u ≡ w
+
+inductive EqCom : Com → Com → Prop
+  | force {v w : Val} : v ≡ w → force v ≡ force w
+  | lam {m n : Com} : m ≡ n → lam m ≡ lam n
+  | app {m n : Com} {v w : Val} : m ≡ n → v ≡ w → app m v ≡ app n w
+  | ret {v w : Val} : v ≡ w → ret v ≡ ret w
+  | letin {n₁ n₂ m₁ m₂ : Com} : m₁ ≡ n₁ → m₂ ≡ n₂ → letin m₁ m₂ ≡ letin n₁ n₂
+  | case {v w : Val} {m₁ n₁ m₂ n₂ : Com} : v ≡ w → m₁ ≡ n₁ → m₂ ≡ n₂ → case v m₁ m₂ ≡ case w n₁ n₂
+  | prod {m₁ m₂ n₁ n₂ : Com} : m₁ ≡ n₁ → m₂ ≡ n₂ → prod m₁ m₂ ≡ prod n₁ n₂
+  | fst {m n : Com} : m ≡ n → fst m ≡ fst n
+  | snd {m n : Com} : m ≡ n → snd m ≡ snd n
+  | β {m v} : app (lam m) v ≡ m⦃v⦄
+  | ζ {m v} : letin (ret v) m ≡ m⦃v⦄
+  | ιl {v m₁ m₂} : case (inl v) m₁ m₂ ≡ m₁⦃v⦄
+  | ιr {v m₁ m₂} : case (inr v) m₁ m₂ ≡ m₂⦃v⦄
+  | π {m} : force (thunk m) ≡ m
+  | π1 {m₁ m₂} : fst (prod m₁ m₂) ≡ m₁
+  | π2 {m₁ m₂} : snd (prod m₁ m₂) ≡ m₂
+  | sym {m n : Com} : n ≡ m → m ≡ n
+  | trans {m n p : Com} : m ≡ n → n ≡ p → m ≡ p
+end
+end
+infix:40 "≡" => EqVal
+infix:40 "≡" => EqCom
+
+theorem reflValCom :
+  (∀ {v : Val}, v ≡ v) ∧
+  (∀ {m : Com}, m ≡ m) := by
+  refine ⟨λ {v} ↦ ?val, λ {m} ↦ ?com⟩
+  mutual_induction v, m
+  all_goals constructor <;> assumption
+
+@[refl] theorem EqVal.refl : ∀ {v : Val}, v ≡ v := reflValCom.left
+@[refl] theorem EqCom.refl : ∀ {m : Com}, m ≡ m := reflValCom.right
+
+instance : Trans EqCom EqCom EqCom where
+  trans := .trans
+
+end Eq
 
 open CK Big
 
 /-* CK machine semantics is sound wrt small-step evaluation semantics *-/
 
-theorem congK {m n k} (r : m ⇒ n) : dismantle m k ⇒ dismantle n k := by
+theorem evalCongK {m n k} (r : m ⇒ n) : dismantle m k ⇒ dismantle n k := by
   induction k generalizing m n
   case nil => simp [r]
   case cons f _ ih =>
@@ -122,7 +179,7 @@ theorem stepEval {m n k₁ k₂} (r : ⟨m, k₁⟩ ⤳ ⟨n, k₂⟩) :
   induction r generalizing m n k₁ k₂
   all_goals injection e₁ with em ek₁; subst em ek₁
   all_goals injection e₂ with en ek₂; subst en ek₂
-  case β | ζ | ιl | ιr | π | π1 | π2 => (try simp); left; apply congK; constructor
+  case β | ζ | ιl | ιr | π | π1 | π2 => (try simp); left; apply evalCongK; constructor
   case app | letin | fst | snd => right; rfl
 
 theorem stepEvals {m n k₁ k₂} (r : ⟨m, k₁⟩ ⤳⋆ ⟨n, k₂⟩) : dismantle m k₁ ⇒⋆ dismantle n k₂ := by
@@ -147,29 +204,29 @@ theorem stepBig {m n k} (r : m ⇓ n) : ⟨m, k⟩ ⤳⋆ ⟨n, k⟩ := by
   case ιl ih => exact .trans .ιl ih
   case ιr ih => exact .trans .ιr ih
   case β n t m v _ _ ih₁ ih₂ =>
-    calc ⟨.app n v, k⟩
-      _ ⤳  ⟨n, .app v :: k⟩      := .app
-      _ ⤳⋆ ⟨.lam m, .app v :: k⟩ := ih₁
-      _ ⤳  ⟨m⦃v⦄, k⟩             := .β
-      _ ⤳⋆ ⟨t, k⟩                := ih₂
+    calc ⟨app n v, k⟩
+      _ ⤳  ⟨n, .app v :: k⟩     := .app
+      _ ⤳⋆ ⟨lam m, .app v :: k⟩ := ih₁
+      _ ⤳  ⟨m⦃v⦄, k⟩            := .β
+      _ ⤳⋆ ⟨t, k⟩               := ih₂
   case ζ n t v m _ _ ih₁ ih₂ =>
-    calc ⟨.letin n m, k⟩
-      _ ⤳  ⟨n, .letin m :: k⟩      := .letin
-      _ ⤳⋆ ⟨.ret v, .letin m :: k⟩ := ih₁
-      _ ⤳  ⟨m⦃v⦄, k⟩               := .ζ
-      _ ⤳⋆ ⟨t, k⟩                  := ih₂
+    calc ⟨letin n m, k⟩
+      _ ⤳  ⟨n, .letin m :: k⟩     := .letin
+      _ ⤳⋆ ⟨ret v, .letin m :: k⟩ := ih₁
+      _ ⤳  ⟨m⦃v⦄, k⟩              := .ζ
+      _ ⤳⋆ ⟨t, k⟩                 := ih₂
   case π1 n t m₁ m₂ _ _ ih₁ ih₂ =>
-    calc ⟨.fst n, k⟩
-      _ ⤳  ⟨n, .fst :: k⟩           := .fst
-      _ ⤳⋆ ⟨.prod m₁ m₂, .fst :: k⟩ := ih₁
-      _ ⤳  ⟨m₁, k⟩                  := .π1
-      _ ⤳⋆ ⟨t, k⟩                   := ih₂
+    calc ⟨fst n, k⟩
+      _ ⤳  ⟨n, .fst :: k⟩          := .fst
+      _ ⤳⋆ ⟨prod m₁ m₂, .fst :: k⟩ := ih₁
+      _ ⤳  ⟨m₁, k⟩                 := .π1
+      _ ⤳⋆ ⟨t, k⟩                  := ih₂
   case π2 n t m₁ m₂ _ _ ih₁ ih₂ =>
-    calc ⟨.snd n, k⟩
-      _ ⤳  ⟨n, .snd :: k⟩           := .snd
-      _ ⤳⋆ ⟨.prod m₁ m₂, .snd :: k⟩ := ih₁
-      _ ⤳  ⟨m₂, k⟩                  := .π2
-      _ ⤳⋆ ⟨t, k⟩                   := ih₂
+    calc ⟨snd n, k⟩
+      _ ⤳  ⟨n, .snd :: k⟩          := .snd
+      _ ⤳⋆ ⟨prod m₁ m₂, .snd :: k⟩ := ih₁
+      _ ⤳  ⟨m₂, k⟩                 := .π2
+      _ ⤳⋆ ⟨t, k⟩                  := ih₂
 
 /-* CK machine is complete wrt small-step evaluation via big-step *-/
 
@@ -203,3 +260,26 @@ theorem bigTerminal {t} (h : isTerminal t) : t ⇓ t := by
 
 theorem evalStep {m t} (h : isTerminal t) (r : m ⇒⋆ t) : ⟨m, []⟩ ⤳⋆ ⟨t, []⟩ :=
   stepBig (evalBigs r (bigTerminal h))
+
+/-* CK machine is sound wrt equational theory *-/
+
+theorem eqCongK {m n : Com} {k} (e : m ≡ n) : dismantle m k ≡ dismantle n k := by
+  induction k generalizing m n
+  case nil => simp [e]
+  case cons f _ ih =>
+    cases f <;> (apply ih; constructor)
+    all_goals first | assumption | rfl
+
+theorem stepEq {m n k₁ k₂} (r : ⟨m, k₁⟩ ⤳ ⟨n, k₂⟩) : dismantle m k₁ ≡ dismantle n k₂ := by
+  cases r
+  case app | letin | fst | snd => rfl
+  all_goals (try simp); apply eqCongK; constructor
+
+theorem stepsEq {m n k₁ k₂} (r : ⟨m, k₁⟩ ⤳⋆ ⟨n, k₂⟩) : dismantle m k₁ ≡ dismantle n k₂ := by
+  generalize e₁ : (m, k₁) = ck₁ at r
+  generalize e₂ : (n, k₂) = ck₂ at r
+  induction r generalizing m n k₁ k₂
+  case refl => subst e₁; injection e₂ with em ek; subst em ek; rfl
+  case trans ck _ r _ ih => subst e₁ e₂; exact .trans (stepEq r) (ih rfl rfl)
+
+theorem stepsEqNil {m n} (r : ⟨m, []⟩ ⤳⋆ ⟨n, []⟩) : m ≡ n := stepsEq r
